checkpoint

theories/machine_run.v
@@ -73,3 +73,61 @@ Proof.
       econstructor. cbn. apply Hc. } }
 Qed.
 
+Fixpoint machine_run_conf `{MachineParameters} (fuel: nat) (c: Conf): Conf :=
+  match fuel with
+  | 0 => c
+  | S fuel =>
+    match c with
+    | (Failed, φ) => c
+    | (Halted, _) => c
+    | (NextI, φ) => machine_run_conf fuel (Executable, φ)
+    | (Executable, (r, m)) =>
+      let pc := r !r! PC in
+      if isCorrectPCb pc then (
+        let a := match pc with
+                 | inl _ => top (* dummy *)
+                 | inr (_, _, _, _, a) => a
+                 end in
+        let i := decodeInstrW (m !m! a) in
+        let c' := exec i (r, m) in
+        machine_run_conf fuel (c'.1, c'.2)
+      ) else (
+        (Failed, (r, m))
+      )
+    end
+  end.
+
+Lemma machine_run_conf_correct `{MachineParameters} fuel cf (φ: ExecConf) cf' φ':
+  machine_run_conf fuel (cf, φ) = (cf', φ') →
+  rtc erased_step
+      ([Seq (Instr cf)], φ)
+      ([Seq (Instr cf')], φ').
+Proof.
+  revert cf cf' φ φ'. induction fuel.
+  { cbn. inversion 1. eapply rtc_refl. }
+  { cbn. intros ? ? [r m] φ' Hc.
+    destruct cf; simplify_eq.
+    destruct (isCorrectPCb (r !r! PC)) eqn:HPC.
+    { apply isCorrectPCb_isCorrectPC in HPC.
+      destruct (r !r! PC) as [|c] eqn:Hr; [by inversion HPC|].
+      destruct_cap c.
+      eapply IHfuel in Hc as Hc.
+      eapply rtc_l. unfold erased_step. exists [].
+      eapply step_atomic with (t1:=[]). 1,2: reflexivity. cbn.
+      eapply ectx_language.Ectx_step with (K:=[SeqCtx]). 1,2: reflexivity.
+      constructor. eapply step_exec_instr; eauto. rewrite Hr //.
+      apply Hc. }
+    { simplify_eq. apply isCorrectPCb_nisCorrectPC in HPC.
+      eapply rtc_l. unfold erased_step. exists [].
+      eapply step_atomic with (t1:=[]). 1,2: reflexivity. cbn.
+      eapply ectx_language.Ectx_step with (K:=[SeqCtx]). 1,2: reflexivity. cbn.
+      constructor. eapply step_exec_fail; eauto.
+      eapply rtc_refl. }
+    { eapply rtc_refl. }
+    { eapply rtc_refl. }
+    { apply IHfuel in Hc as Hc.
+      eapply rtc_l. exists [].
+      eapply step_atomic with (t1:=[]). 1,2: reflexivity. cbn.
+      eapply ectx_language.Ectx_step with (K:=[]). 1,2: reflexivity. cbn.
+      econstructor. cbn. apply Hc. } }
+Qed.
